src/cbor/pulse/raw/everparse/CBOR.Pulse.Raw.EverParse.Serialize.fsti
@@ -1,1 +1,43 @@
 module CBOR.Pulse.Raw.EverParse.Serialize
+
+open Pulse.Lib.Pervasives
+open CBOR.Spec.Raw.Base
+open CBOR.Spec.Raw.Format
+open CBOR.Pulse.Raw.EverParse.Match
+open CBOR.Pulse.Raw.EverParse.Type
+module SZ = FStar.SizeT
+module S = Pulse.Lib.Slice
+module U8 = FStar.UInt8
+
+val cbor_serialize
+  (f64: squash SZ.fits_u64)
+  (x: cbor_raw)
+  (output: S.slice U8.t)
+  (#y: Ghost.erased raw_data_item)
+  (#pm: perm)
+: stt SZ.t
+    (exists* v . cbor_raw_match pm x y ** pts_to output v ** pure (Seq.length (serialize_cbor y) <= SZ.v (S.len output)))
+    (fun res -> exists* v . cbor_raw_match pm x y ** pts_to output v ** pure (
+      let s = serialize_cbor y in
+      SZ.v res == Seq.length s /\
+      (exists v' . v `Seq.equal` (s `Seq.append` v'))
+    ))
+
+let cbor_size_post
+  (bound: SZ.t)
+  (y: raw_data_item)
+  (res: SZ.t)
+: Tot prop
+= let s = Seq.length (serialize_cbor y) in
+  (SZ.v res == 0 <==> s > SZ.v bound) /\
+  (SZ.v res > 0 ==> SZ.v res == s)
+
+val cbor_size
+  (f64: squash SZ.fits_u64)
+  (x: cbor_raw)
+  (bound: SZ.t)
+  (#y: Ghost.erased raw_data_item)
+  (#pm: perm)
+: stt SZ.t
+    (cbor_raw_match pm x y)
+    (fun res -> cbor_raw_match pm x y ** pure (cbor_size_post bound y res))
